fstar/new/TreeSync.fst
@@ -4,6 +4,7 @@ open Lib.Array
 open Lib.Maths
 open Lib.ByteSequence
 open Utils
+open Tree
 
 //Theophile: these types are needed on my computer
 let bytes_t = bytes
@@ -52,50 +53,55 @@ let mk_initial_leaf_package (c:credential_t) =
 
 
 (** Definition of a Node package *)
-type direction_t = | Left | Right
+//type direction_t = | Left | Right
 type node_package_t = {
   np_version: nat;
-  np_content_dir: direction_t;
+  np_content_dir: direction;
   np_unmerged_leafs: list nat;
   np_content: pub_bytes_t;
 }
 
 
 (** Tree and Paths definitions *)
-type index_n (l:nat) = x:nat{x < pow2 l}
+//type index_n (l:nat) = x:nat{x < pow2 l}
 type level_n = nat
 
-type tree_t (l:level_n) =
- | Leaf: actor:credential_t{l=0} -> olp:option leaf_package_t -> tree_t l
- | Node: actor:credential_t{l>0} -> onp:option node_package_t ->
-         left:tree_t (l-1) -> right:tree_t (l-1) -> tree_t l
+type treesync (l:level_n) (n:tree_size l) = tree l n (credential_t & option leaf_package_t) (credential_t & option node_package_t)
+type pathsync (l:level_n) (n:tree_size l) (i:leaf_index n) = path l n i (option leaf_package_t) (option node_package_t)
+//type tree_t (l:level_n) =
+// | Leaf: actor:credential_t{l=0} -> olp:option leaf_package_t -> tree_t l
+// | Node: actor:credential_t{l>0} -> onp:option node_package_t ->
+//         left:tree_t (l-1) -> right:tree_t (l-1) -> tree_t l
 
-type path_t (l:level_n) =
- | PLeaf: olp:option leaf_package_t{l=0} -> path_t l
- | PNode: onp:option node_package_t{l>0} ->
-	       next:path_t (l-1) -> path_t l
+//type path_t (l:level_n) =
+// | PLeaf: olp:option leaf_package_t{l=0} -> path_t l
+// | PNode: onp:option node_package_t{l>0} ->
+//	       next:path_t (l-1) -> path_t l
 
 (** Operations on the state *)
 type operation_t = {
   op_levels: level_n;
-  op_index: index_n op_levels;
+  op_treesize: tree_size op_levels;
+  op_index: leaf_index op_treesize;
   op_actor: credential_t;
-  op_path: path_t op_levels;
+  op_path: pathsync op_levels op_treesize op_index;
 }
 
 (** TreeSync state and accessors *)
 type state_t = {
   st_group_id: nat;
   st_levels: level_n;
-  st_tree: tree_t st_levels;
+  st_treesize: tree_size st_levels;
+  st_tree: treesync st_levels st_treesize;
   st_version: nat;
-  st_initial_tree: tree_t st_levels;
+  st_initial_tree: treesync st_levels st_treesize;
   st_transcript: Seq.seq operation_t;
 }
 
-val mk_initial_state: gid:nat -> l:level_n -> tree_t l -> Tot state_t
-let mk_initial_state gid l t = {
+val mk_initial_state: gid:nat -> l:level_n -> n:tree_size l -> treesync l n -> Tot state_t
+let mk_initial_state gid l n t = {
   st_group_id = gid; st_levels = l;
+  st_treesize = n;
   st_tree = t; st_version = 0;
   st_initial_tree = t;
   st_transcript = empty;}
@@ -109,81 +115,90 @@ let max_size st = pow2 st.st_levels
 val epoch: state_t -> nat
 let epoch st = st.st_version
 
-type index_t (st:state_t) = i:nat{i < max_size st}
+type index_t (st:state_t) = i:nat{i < st.st_treesize}
 
 
 (** Membership *)
 type member_array_t (sz:nat) = a:array (option credential_t){length a = sz}
 
-let rec tree_membership (l:nat) (t:tree_t l): member_array_t (pow2 l) =
+let rec tree_membership (#l:nat) (#n:tree_size l) (t:treesync l n): member_array_t n =
   match t with
-  | Leaf _ olp ->
+  | TLeaf (_, olp) ->
     (match olp with
     | None -> singleton None
     | Some lp -> singleton (Some lp.lp_credential))
-  | Node _ _ left right -> append (tree_membership (l-1) left)
-				 (tree_membership (l-1) right)
+  | TSkip _ t' -> tree_membership t'
+  | TNode (_,_) left right -> append (tree_membership left)
+				 (tree_membership right)
 
-val membership: st:state_t -> member_array_t (max_size st)
-let membership st = tree_membership st.st_levels st.st_tree
+val membership: st:state_t -> member_array_t (st.st_treesize)
+let membership st = tree_membership st.st_tree
 
 
 (** Auxiliary tree functions *)
-let dual (d:direction_t) : direction_t =
+let dual (d:direction) : direction =
   match d with
   | Left -> Right
   | Right -> Left
 
-let child_index (l:pos) (i:index_n l) : index_n (l-1) & direction_t =
-  if i < pow2 (l - 1) then (i, Left) else (i-pow2 (l-1), Right)
+//let child_index (l:pos) (i:index_n l) : index_n (l-1) & direction_t =
+//  if i < pow2 (l - 1) then (i, Left) else (i-pow2 (l-1), Right)
 
-let order_subtrees dir (l,r) = if dir = Left then (l,r) else (r,l)
+//let order_subtrees dir (l,r) = if dir = Left then (l,r) else (r,l)
 
 
 (** Create a new tree from a member array *)
-val create_tree: l:level_n -> actor:credential_t ->
-		 init:member_array_t (pow2 l) ->
-		 t:tree_t l{tree_membership l t == init}
+val create_tree: l:level_n -> n:tree_size l -> actor:credential_t ->
+		 init:member_array_t n ->
+		 t:treesync l n{tree_membership t == init}
 
-let rec create_tree (l:level_n) (actor:credential_t) (init:member_array_t (pow2 l)) =
+let rec create_tree (l:level_n) (n:tree_size l) (actor:credential_t) (init:member_array_t n) =
   if l = 0 then
     match init.[0] with
-    | None -> Leaf actor None
-    | Some c -> Leaf actor (Some (mk_initial_leaf_package c))
+    | None -> TLeaf (actor, None)
+    | Some c -> TLeaf (actor, (Some (mk_initial_leaf_package c)))
   else
-    let init_l,init_r = split init (pow2 (l-1)) in
-    let left = create_tree (l-1) actor init_l in
-    let right = create_tree (l-1) actor init_r in
-    Node actor None left right
+    if n <= (pow2 (l-1)) then
+      TSkip _ (create_tree (l-1) n actor init)
+    else
+      let init_l,init_r = split init (pow2 (l-1)) in
+      let left = create_tree (l-1) (pow2 (l-1)) actor init_l in
+      let right = create_tree (l-1) (n - pow2 (l-1)) actor init_r in
+      TNode (actor, None) left right
 
 
 (** Apply a path to a tree *)
-let rec apply_path (l:level_n) (i:nat{i<pow2 l}) (a:credential_t)
-                   (t:tree_t l) (p:path_t l) : tree_t l =
+let rec apply_path (#l:level_n) (#n:tree_size l) (#i:leaf_index n) (a:credential_t)
+                   (t:treesync l n) (p:pathsync l n i) : treesync l n =
   match t,p with
-  | Leaf _ m, PLeaf m' -> Leaf a m'
-  | Node _ _ left right, PNode onp next ->
-     let (j,dir) = child_index l i in
+  | TLeaf (_, m), PLeaf m' -> TLeaf (a, m')
+  | TSkip _ t', PSkip _ p' -> TSkip _ (apply_path a t' p')
+  | TNode (_, _) left right, PNode onp next ->
+     let (|dir,_|) = child_index l i in
      if dir = Left
-     then Node a onp (apply_path (l-1) j a left next) right
-     else Node a onp left (apply_path (l-1) j a right next)
+     then TNode (a, onp) (apply_path a left next) right
+     else TNode (a, onp) left (apply_path a right next)
 
 
 (** Create a blank path after modifying a leaf *)
-let rec blank_path (l:level_n) (i:index_n l) (oc:option credential_t) : path_t l =
+let rec blank_path (l:level_n) (n:tree_size l) (i:leaf_index n) (oc:option credential_t) : pathsync l n i =
   if l = 0 then
     match oc with
     | None -> PLeaf None
     | Some c -> PLeaf (Some (mk_initial_leaf_package c))
-  else let (j,dir) = child_index l i in
-    PNode None (blank_path (l-1) j oc)
+  else if n <= pow2 (l-1) then
+    PSkip _ (blank_path (l-1) n i oc)
+  else
+    let (|dir,j|) = child_index l i in
+    PNode None (blank_path (l-1) (if dir = Left then (pow2 (l-1)) else (n - (pow2 (l-1)))) j oc)
 
-let rec unmerged_path (#l:level_n) (leaf_index:index_n l) (t:tree_t l) (cred:credential_t): path_t l =
+let rec unmerged_path (#l:level_n) (#n:tree_size l) (leaf_index:leaf_index n) (t:treesync l n) (cred:credential_t): pathsync l n leaf_index =
   match t with
-  | Leaf _ _ ->
+  | TLeaf (_, _) ->
     PLeaf (Some (mk_initial_leaf_package cred))
-  | Node _ onp left right ->
-    let (new_leaf_index, dir) = child_index l leaf_index in
+  | TSkip _ t' -> PSkip _ (unmerged_path leaf_index t' cred)
+  | TNode (_, onp) left right ->
+    let (|dir, new_leaf_index|) = child_index l leaf_index in
     let (child, _) = order_subtrees dir (left, right) in
     let path_next = unmerged_path new_leaf_index child cred in
     match onp with
@@ -200,16 +215,17 @@ let rec unmerged_path (#l:level_n) (leaf_index:index_n l) (t:tree_t l) (cred:cre
 
 (** Create an operation that modifies the group state *)
 val mk_operation: st:state_t -> actor:credential_t
-  -> i:index_t st -> p:path_t st.st_levels
+  -> i:index_t st -> p:pathsync st.st_levels st.st_treesize i
   -> Tot (option operation_t)
 
 let mk_operation st actor i p =
-  match (membership st).[i], (PLeaf?.olp p) with
+  match (membership st).[i], (PLeaf?.data p) with
   | _ -> None
   | Some mc, Some lp ->
   if mc = lp.lp_credential then None
   else
     Some ({op_levels = st.st_levels;
+           op_treesize = st.st_treesize;
            op_index = i;
            op_actor = actor;
            op_path = p;})
@@ -223,8 +239,8 @@ let create gid sz init =
   match init.[0], log2 sz with
   | _ -> None
   | Some actor,Some l ->
-    let t = create_tree l actor init in
-    let st = mk_initial_state gid l t in
+    let t = create_tree l sz actor init in
+    let st = mk_initial_state gid l sz t in
     Some ({st with st_initial_tree = t;
                    st_transcript = bytes_empty})
 
@@ -234,9 +250,9 @@ val apply: state_t -> operation_t
   -> Tot (option state_t)
 
 let apply st op =
-  if op.op_levels <> st.st_levels then None
+  if op.op_levels <> st.st_levels || op.op_treesize <> st.st_treesize then None
   else
-    let nt = apply_path op.op_levels op.op_index op.op_actor st.st_tree op.op_path in
+    let nt = apply_path op.op_actor st.st_tree op.op_path in
     Some ({ st with st_version = st.st_version + 1; st_tree = nt;
             st_transcript = Seq.snoc st.st_transcript op})
 
@@ -261,7 +277,7 @@ val remove: st:state_t -> actor:credential_t -> i:index_t st
   -> Tot (option (operation_t & state_t))
 
 let remove st actor i =
-  let p = blank_path st.st_levels i None in
+  let p = blank_path st.st_levels st.st_treesize i None in
   match mk_operation st actor i p with
   | None -> None
   | Some op ->
