fstar/new/TreeSyncTreeKEMBinder.fst
@@ -4,6 +4,7 @@ open Lib.ByteSequence
 open Crypto
 open NetworkTypes
 open Parser
+open Tree
 module TS = TreeSync
 module TK = TreeKEM
 open Lib.Result
@@ -20,16 +21,6 @@ let secret_to_pub b =
   let open Lib.IntTypes in
   Seq.seq_of_list (List.Tot.map (fun x -> byte (v x)) (Seq.seq_to_list b))
 
-//TODO They should be the same type
-let dir_ts_to_tk (dir:TS.direction_t) =
-  match dir with
-  | TS.Left -> TK.Left
-  | TS.Right -> TK.Right
-let dir_tk_to_ts (dir:TK.direction) =
-  match dir with
-  | TK.Left -> TS.Left
-  | TK.Right -> TS.Right
-
 let encrypted_path_secret_nt_to_tk (cs:ciphersuite) (x:hpke_ciphertext_nt): result (TK.path_secret_ciphertext cs) =
   if not (Seq.length x.hcn_kem_output = hpke_kem_output_length cs) then
     fail "encrypted_path_secret_nt_to_tk: kem_output has wrong length"
@@ -39,46 +30,42 @@ let encrypted_path_secret_nt_to_tk (cs:ciphersuite) (x:hpke_ciphertext_nt): resu
       TK.ciphertext = x.hcn_ciphertext;
     })
 
-let nat_to_index_l (l:nat) (x:nat): result (TK.index_l l) =
-  if not (x < pow2 l) then
-    fail "nat_to_index_l: unmerged leaf index is too big"
-  else
-    return x
-
-val treesync_to_treekem: #l:nat -> cs:ciphersuite -> TS.tree_t l -> result (TK.tree cs l)
-let rec treesync_to_treekem #l cs t =
+val treesync_to_treekem: #l:nat -> #n:tree_size l -> cs:ciphersuite -> TS.treesync l n -> result (TK.treekem cs l n)
+let rec treesync_to_treekem #l #n cs t =
   match t with
-  | TS.Leaf _ None ->
-    return (TK.Leaf None)
-  | TS.Leaf _ (Some lp) ->
+  | TLeaf (_, None) ->
+    return (TLeaf None)
+  | TLeaf (_, (Some lp)) ->
     pk <-- from_option "treesync_to_treekem: Couldn't parse HPKEPublicKey"
       ((ps_to_pse ps_hpke_public_key).parse_exact (pub_to_secret lp.TS.lp_content));
     if Seq.length pk = hpke_public_key_length cs then
-      return (TK.Leaf (Some ({TK.mi_public_key = pk; TK.mi_version = lp.TS.lp_version})))
+      return (TLeaf (Some ({TK.mi_public_key = pk; TK.mi_version = lp.TS.lp_version})))
     else
       fail "treesync_to_treekem: public key has wrong length"
-  | TS.Node _ onp left right -> begin
+  | TSkip _ t' ->
+    result <-- treesync_to_treekem cs t';
+    return (TSkip _ result)
+  | TNode (_, onp) left right -> begin
     tk_left <-- treesync_to_treekem cs left;
     tk_right <-- treesync_to_treekem cs right;
     match onp with
     | None ->
-      return (TK.Node None tk_left tk_right)
+      return (TNode None tk_left tk_right)
     | Some np ->
       content <-- from_option "treesync_to_treekem: Couldn't parse UpdatePathNode"
         ((ps_to_pse ps_update_path_node).parse_exact (pub_to_secret np.TS.np_content));
       path_secret_ciphertext <-- mapM (encrypted_path_secret_nt_to_tk cs) (Seq.seq_to_list content.upnn_encrypted_path_secret);
-      unmerged_leafs <-- mapM (nat_to_index_l l) (np.TS.np_unmerged_leafs);
       if not (Seq.length content.upnn_public_key = hpke_public_key_length cs) then
         fail ""
       else (
-        let kp: TK.key_package cs l = {
+        let kp: TK.key_package cs = {
           TK.kp_public_key = content.upnn_public_key;
           TK.kp_version = np.TS.np_version;
-          TK.kp_unmerged_leafs = unmerged_leafs;
-          TK.kp_path_secret_from = dir_ts_to_tk (np.TS.np_content_dir);
+          TK.kp_unmerged_leafs = np.TS.np_unmerged_leafs;
+          TK.kp_path_secret_from = (np.TS.np_content_dir);
           TK.kp_path_secret_ciphertext = path_secret_ciphertext;
         } in
-        return (TK.Node (Some kp) tk_left tk_right)
+        return (TNode (Some kp) tk_left tk_right)
       )
   end
 
@@ -94,16 +81,19 @@ let encrypted_path_secret_tk_to_nt (#cs:ciphersuite) (x:TK.path_secret_ciphertex
     })
 
 
-val treekem_to_treesync: #l:nat -> #cs:ciphersuite -> TS.credential_t -> TK.path cs l -> result (TS.path_t l)
+val treekem_to_treesync: #l:nat -> #n:tree_size l -> #i:leaf_index n -> #cs:ciphersuite -> TS.credential_t -> TK.pathkem cs l n i -> result (TS.pathsync l n i)
 let rec treekem_to_treesync #l #cs cred p =
   match p with
-  | TK.PLeaf mi ->
-    return (TS.PLeaf (Some ({
+  | PLeaf mi ->
+    return (PLeaf (Some ({
       TS.lp_credential = cred;
       TS.lp_version = mi.TK.mi_version;
       TS.lp_content = secret_to_pub (ps_hpke_public_key.serialize mi.TK.mi_public_key);
     })))
-  | TK.PNode kp p_next ->
+  | PSkip _ p' ->
+    result <-- treekem_to_treesync cred p';
+    return (PSkip _ result)
+  | PNode kp p_next ->
     next <-- treekem_to_treesync cred p_next;
     ciphertexts <-- mapM encrypted_path_secret_tk_to_nt kp.TK.kp_path_secret_ciphertext;
     if not (byte_length ps_hpke_ciphertext ciphertexts < pow2 16) then
@@ -116,9 +106,9 @@ let rec treekem_to_treesync #l #cs cred p =
       }) in
       let np = ({
         TS.np_version = kp.TK.kp_version;
-        TS.np_content_dir = dir_tk_to_ts kp.TK.kp_path_secret_from;
-        TS.np_unmerged_leafs = List.Tot.map (fun (x:TK.index_l l) -> (x<:nat)) kp.TK.kp_unmerged_leafs;
+        TS.np_content_dir = kp.TK.kp_path_secret_from;
+        TS.np_unmerged_leafs = kp.TK.kp_unmerged_leafs;
         TS.np_content = secret_to_pub np_content;
       }) in
-      return (TS.PNode (Some np) next)
+      return (PNode (Some np) next)
     end
